strotoimax_part: spec and proof for memory loads and stores of strtoimax

doc/tutorial/C/easy_ptr.c
@@ -1,7 +1,0 @@
-int ptr_test(char *ptr1, char *ptr2) {
-  if (ptr1 <= ptr2) {
-    return 1;
-  } else {
-    return 2;
-  }
-}
