doc/tutorial/C/ptrs.c
@@ -5,9 +5,10 @@ int ptr_test(char *ptr1, char **ptr2) {
   return 0;
 }
 
-int ptr_test_2(char *ptr1, char **ptr2) {
-  if (ptr1 <= *ptr2) {
-    return 0;
-  }
-  return 2;
+int ptr_test_2 (char *ptr1, char *ptr2) {
+  if (ptr1 <= ptr2) {
+    return 1;
+  } else {
+    return 2;
+  } 
 }
