doc/tutorial/C/strtoimax_part.c
@@ -1,0 +1,22 @@
+ int asn_strtoimax_lim(const char *str, const char **end, int *intp) {
+
+    int sign = 1;
+
+    if(str >= *end) return 0;
+
+    switch(*str) {
+    case '-':
+        sign = -1;
+        /* FALL THROUGH */
+    case '+':
+        str++;
+        if(str >= *end) {
+            *end = str;
+            return 1;
+        }
+    }
+
+    *end = str;
+    *intp = sign;
+    return 2;
+}
