doc/tutorial/ptrs_vst.v
@@ -64,65 +64,241 @@ Qed.
 
 Definition ptr_test_2_fun_spec (ofs1 ofs2 : ptrofs) :=
   if Ptrofs.unsigned ofs1 <=? Ptrofs.unsigned ofs2
-  then 0
+  then 1
   else 2.
 
-  
+
 Definition ptr_test_2_spec : ident * funspec :=
   DECLARE _ptr_test_2
-    WITH sh: share,
-         b1 : block, b2 : block, b3 : block,
-         ofs1 : ptrofs, ofs2 : ptrofs, ofs3 : ptrofs,
-         c1 : int, c2 : int
-    PRE [_ptr1 OF (tptr tschar), _ptr2 OF (tptr (tptr tschar))]
-      PROP (readable_share sh;
-            b1 = b3)
-      LOCAL (temp _ptr1 (Vptr b1 ofs1); 
-             temp _ptr2 (Vptr b2 ofs2))
-      SEP (data_at sh  (tschar) (Vint c1) (Vptr b1 ofs1);  
-           data_at sh  (tschar) (Vint c2) (Vptr b3 ofs3);
-           data_at sh (tptr tschar) (Vptr b3 ofs3) (Vptr b2 ofs2))
+    WITH b : block, ptr1 : ptrofs, ptr2 : ptrofs,
+         sh : share, ch1 : Z, ch2 : Z
+    PRE [_ptr1 OF (tptr tschar), _ptr2 OF (tptr tschar)]
+      PROP(readable_share sh)
+      LOCAL(temp _ptr1 (Vptr b ptr1);
+            temp _ptr2 (Vptr b ptr2))
+      SEP(data_at sh tschar (Vint (Int.repr ch1)) (Vptr b ptr1);
+          data_at sh tschar (Vint (Int.repr ch2)) (Vptr b ptr2))
     POST [tint]
-      PROP ()
-      LOCAL (temp ret_temp ((Vint ∘ Int.repr)(ptr_test_2_fun_spec ofs1 ofs3)))
-      SEP (data_at sh (tschar) (Vint c1) (Vptr b1 ofs1);  
-           data_at sh (tschar) (Vint c2) (Vptr b3 ofs3);
-           data_at sh (tptr tschar) (Vptr b3 ofs3) (Vptr b2 ofs2)).
+      PROP()
+      LOCAL(temp ret_temp (Vint (Int.repr (ptr_test_2_fun_spec ptr1 ptr2))))
+      SEP(data_at sh tschar (Vint (Int.repr ch1)) (Vptr b ptr1);
+          data_at sh tschar (Vint (Int.repr ch2)) (Vptr b ptr2)).
 
-Lemma body_str_test_2: semax_body Vprog Gprog f_ptr_test ptr_test_spec.
+Definition Gprog_2 := ltac:(with_library prog [ptr_test_2_spec]).
+
+Lemma typed_true_ptr_le : forall b ptr1 ptr2, 
+        typed_true tint (force_val (sem_cmp_pp Cle (Vptr b ptr1) (Vptr b ptr2))) ->
+        Ptrofs.unsigned ptr1 <=? Ptrofs.unsigned ptr2 = true.
+Proof.
+  intros.
+  unfold typed_true, force_val, sem_cmp_pp in H.
+  unfold Archi.ptr64, strict_bool_val in H.
+  simpl in H.
+  destruct eq_block in H; [simpl in H|contradiction].
+  unfold negb, Ptrofs.ltu in H.
+  destruct zlt in H; simpl in H; try discriminate.
+  apply Z.ge_le in g.
+  apply Zle_imp_le_bool.
+  assumption.
+Qed.
+
+Lemma typed_false_ptr_le : forall b ptr1 ptr2, 
+        typed_false tint (force_val (sem_cmp_pp Cle (Vptr b ptr1) (Vptr b ptr2))) ->
+        Ptrofs.unsigned ptr2 <? Ptrofs.unsigned ptr1 = true.
+Proof.
+  intros.
+  unfold typed_false, force_val, sem_cmp_pp in H.
+  unfold Archi.ptr64, strict_bool_val in H.
+  simpl in H.
+  destruct eq_block in H; [simpl in H|contradiction].
+  unfold negb, Ptrofs.ltu in H.
+  destruct zlt in H; simpl in H; try discriminate.
+  apply Fcore_Zaux.Zlt_bool_true.
+  assumption.
+Qed.
+
+Lemma body_ptr_test_2: semax_body Vprog Gprog_2 f_ptr_test_2 ptr_test_2_spec.
 Proof.
   start_function.
-  forward.
   forward_if.
   unfold test_order_ptrs.
   unfold sameblock.
   destruct peq; [simpl|contradiction].
-  eapply andp_right.
-  - assert ( data_at sh tschar (Vint c1) (Vptr b1 ofs1) *
-             data_at sh tschar (Vint c2) (Vptr b1 ofs3) *
-             data_at sh (tptr tschar) (Vptr b1 ofs3) (Vptr b2 ofs2)
-                     |-- valid_pointer (Vptr b1 ofs1)) by entailer!.
-    pose proof (valid_pointer_weak (Vptr b1 ofs1)).
-    eapply derives_trans with (Q := valid_pointer (Vptr b1 ofs1)).
-    eassumption.
-    eapply (valid_pointer_weak (Vptr b1 ofs1)).
-  - erewrite sepcon_assoc.
-    assert ( 
-        data_at sh tschar (Vint c2) (Vptr b1 ofs3) *
-        data_at sh tschar (Vint c1) (Vptr b1 ofs1) *
-        data_at sh (tptr tschar) (Vptr b1 ofs3) (Vptr b2 ofs2)
-                |-- valid_pointer (Vptr b1 ofs3)) by entailer!.
-    pose proof (valid_pointer_weak (Vptr b1 ofs3)).
-    eapply derives_trans with (Q := valid_pointer (Vptr b1 ofs3)).
+  apply andp_right.
+  -
+    assert (data_at sh tschar (Vint (Int.repr ch1)) (Vptr b ptr1) * 
+            data_at sh tschar (Vint (Int.repr ch2)) (Vptr b ptr2) 
+                    |-- valid_pointer (Vptr b ptr1)) by entailer!.
+    pose proof (valid_pointer_weak (Vptr b ptr1)).
+    apply derives_trans with (Q := valid_pointer (Vptr b ptr1)); assumption.
+  -
+    assert (data_at sh tschar (Vint (Int.repr ch1)) (Vptr b ptr1) * 
+            data_at sh tschar (Vint (Int.repr ch2)) (Vptr b ptr2) 
+                    |-- valid_pointer (Vptr b ptr2)) by entailer!.
+    pose proof (valid_pointer_weak (Vptr b ptr2)).
+    apply derives_trans with (Q := valid_pointer (Vptr b ptr2)); assumption.
+  - forward.
+    pose proof typed_true_ptr_le b ptr1 ptr2 H.
+    unfold ptr_test_2_fun_spec.
+    rewrite H4.
+    entailer!.
+  - forward.
+    pose proof typed_false_ptr_le b ptr1 ptr2 H.
+    unfold ptr_test_2_fun_spec.
+    rewrite Z.leb_antisym.
+    rewrite H4.
+    simpl.
+    entailer!.
+Qed.  
+  
+Require Import strtoimax_part.
+
+(* int asn_strtoimax_lim(const char *str, const char **end, int *intp) {
+
+    int sign = 1;
+
+    if(str >= *end) return 0;
+
+    switch( *str) {
+    case '-':
+        sign = -1;
+        /* FALL THROUGH */
+    case '+':
+        str++;
+        if(str >= *end) {
+            *end = str;
+            return 1;
+        }
+    }
+
+    *end = str;
+    *intp = sign;
+    return 2;
+}
+ *)
+
+Definition strtoimax_part_fun_spec (str fin : ptrofs) (ls : list byte) :=
+  if Ptrofs.unsigned fin <=? Ptrofs.unsigned str
+  then 0
+  else       
+    match ls with
+    | [] => 3 
+    | [ch] => if orb (Byte.eq ch (Byte.repr 43)) (Byte.eq ch (Byte.repr 45))
+              then if Ptrofs.unsigned fin <=? Ptrofs.unsigned (Ptrofs.add str Ptrofs.one)
+                   then 1
+                   else 2
+              else 2
+    | _ => 2
+    end. 
+
+Definition strtoimax_part_spec : ident * funspec :=
+  DECLARE _asn_strtoimax_lim
+    WITH str_b : block, str_ofs : ptrofs,
+         end_b : block, end_ofs : ptrofs,
+         end'_b : block, end'_ofs : ptrofs,
+         intp_b : block, intp_ofs : ptrofs,
+         sh : share, sh' : share,
+         contents : list byte,
+         ch : val,
+         sign : val
+    PRE [_str OF (tptr tschar), _end OF (tptr (tptr tschar)), _intp OF (tptr tint)]
+      PROP (readable_share sh; 
+            writable_share sh';
+            str_b = end'_b;
+            (Ptrofs.unsigned str_ofs < Ptrofs.unsigned end'_ofs) ->
+            (Vptr str_b str_ofs <> nullval))
+      LOCAL (temp _str (Vptr str_b str_ofs);
+             temp _end (Vptr end_b end_ofs); 
+             temp _intp (Vptr intp_b intp_ofs))
+      SEP (
+        data_at sh tschar ch (Vptr end'_b end'_ofs);
+           data_at sh (tarray tschar (Zlength contents))
+                   (map Vbyte contents) (Vptr str_b str_ofs);
+           data_at sh' (tptr tschar) (Vptr end'_b end'_ofs) (Vptr end_b end_ofs))
+    POST [tint]
+      PROP()
+      LOCAL (temp ret_temp ((Vint ∘ Int.repr) 
+                           (strtoimax_part_fun_spec str_ofs end'_ofs contents)))
+      SEP (
+        data_at sh tschar ch (Vptr end'_b end'_ofs);
+           data_at sh (tarray tschar (Zlength contents))
+                   (map Vbyte contents) (Vptr str_b str_ofs);
+           let i := strtoimax_part_fun_spec str_ofs end'_ofs contents in
+           if i =? 0 
+           then data_at sh' (tptr tschar) (Vptr end'_b end'_ofs) (Vptr end_b end_ofs)
+           else 
+             if i =? 1 
+             then data_at sh' (tptr tschar) 
+                          (Vptr str_b (Ptrofs.add str_ofs Ptrofs.one))
+                          (Vptr end_b end_ofs) 
+             else 
+               if i =? 2 
+               then
+                 data_at sh' (tptr tschar) 
+                         (Vptr str_b (Ptrofs.add str_ofs Ptrofs.one))
+                         (Vptr end_b end_ofs) *
+                 data_at sh' tint sign (Vptr intp_b intp_ofs)
+               else data_at sh' (tptr tschar) (Vptr end'_b end'_ofs) 
+                                    (Vptr end_b end_ofs)).
+
+Definition Gprog_3 := ltac:(with_library prog [strtoimax_part_spec]).
+
+Lemma body_strtoimax_part : semax_body Vprog Gprog_3 f_asn_strtoimax_lim strtoimax_part_spec.
+  Proof.
+    start_function.
+    repeat forward.
+    forward_if.
+    unfold test_order_ptrs.
+    unfold sameblock.
+    destruct peq; [simpl|contradiction].
+    eapply andp_right.
+    erewrite sepcon_assoc.
+    assert (data_at sh (tarray tschar (Zlength contents)) 
+                    (map Vbyte contents) (Vptr end'_b str_ofs) *
+            data_at sh tschar ch (Vptr end'_b end'_ofs) *
+            data_at sh' (tptr tschar) (Vptr end'_b end'_ofs) (Vptr end_b end_ofs)
+                    |-- valid_pointer (Vptr end'_b str_ofs)).
+    admit. (* need 0 < Zlength contents *) 
+    pose proof (valid_pointer_weak (Vptr end'_b str_ofs)).
+    eapply derives_trans with (Q := valid_pointer (Vptr end'_b str_ofs)).
     erewrite pull_left_special.
     erewrite <- sepcon_assoc.
     eassumption.
-    eapply (valid_pointer_weak (Vptr b1 ofs3)).
-    - forward.
-    - forward.
-Qed.
+    eapply (valid_pointer_weak (Vptr end'_b str_ofs)).
+    assert ( data_at sh tschar ch (Vptr end'_b end'_ofs) *
+             data_at sh (tarray tschar (Zlength contents))
+                     (map Vbyte contents) (Vptr end'_b str_ofs) *
+             data_at sh' (tptr tschar) (Vptr end'_b end'_ofs)
+                     (Vptr end_b end_ofs)
+                     |-- valid_pointer (Vptr end'_b end'_ofs)) by entailer!.
+    pose proof (valid_pointer_weak (Vptr end'_b end'_ofs)).
+    eapply derives_trans with (Q := valid_pointer (Vptr end'_b end'_ofs)).
+    eassumption.
+    eapply (valid_pointer_weak (Vptr end'_b end'_ofs)).
+    forward.
+    entailer!.
+    unfold strtoimax_part_fun_spec.
+    admit. (* true from H1 *)
+    assert (strtoimax_part_fun_spec str_ofs end'_ofs contents =? 0 = true) by admit.
+    (* from H1 *)
+    rewrite H.
+    entailer.
+    
+    Search data_at tarray. 
+    Variable c : byte.
+    Variable tl : list byte.
+    replace (map Vbyte contents) with ([Vbyte c] ++ (map Vbyte tl)).
+    erewrite split2_data_at_Tarray_app with (mid := 1).
+    Intros.
+    Search data_at 1.
+    erewrite data_at_singleton_array_eq.
+    instantiate (1 := Vbyte c).
+    forward.
+    admit.
+
+    
+    
   
-  
-  
+
 
   
